\documentclass{article}
\usepackage{tekvideoexercises}

\begin{document}
Kædereglen
\tableofcontents
\newpage

\begin{exercise}{Differentiering 2 - 01}

Bestem $\frac{d}{dx} (x + 3)^4$.

\answerbox{4 (x + 3)^3}

\hint
Benyt kæde reglen
\[
\frac{d}{dx} f(g(x)) = f'(g(x)) \cdot g'(x)
\]

\hint
Sæt $f(x) = x^4$ og $g(x) = x + 3$ og bestem $f'(x)$ og $g'(x)$.
\[
f'(x) = 4 x^3 \qquad g'(x) = 1
\]

\hint
Indsæt i kædereglen
\[
\frac{d}{dx} (x + 3)^4 = 4 (x + 3)^3 \cdot 1 = 4 (x + 3)^3
\]

\end{exercise}

\begin{exercise}{Differentiering 2 - 02}

Bestem $\frac{d}{dx} e^{2x + x^2}$.

\answerbox{e^{2x + x^2} \cdot (2 + 2x)}

\hint
Benyt kæde reglen
\[
\frac{d}{dx} f(g(x)) = f'(g(x)) \cdot g'(x)
\]

\hint
Sæt $f(x) = e^x$ og $g(x) = 2x + x^2$ og bestem $f'(x)$ og $g'(x)$.
\[
f'(x) = e^x \qquad g'(x) = 2 + 2x
\]

\hint
Indsæt i kædereglen
\[
\frac{d}{dx} e^{2x + x^2} = e^{2x + x^2} \cdot (2 + 2x)
\]

\end{exercise}

\begin{exercise}{Differentiering 2 - 03}
	
	Bestem $\frac{d}{dx} \left(x^2 + 1	\right)^5 $.
	
	\answerbox{10x \cdot \left(x^2 + 1 \right)^4}
	
	\hint
	Benyt kæde reglen
	\[
	\frac{d}{dx} f(g(x)) = f'(g(x)) \cdot g'(x)
	\]
	
	\hint
	Sæt $f(x) = x^5$ og $g(x) = x^2 + 1$ og bestem $f'(x)$ og $g'(x)$.
	\[
	f'(x) = 5x^4  \qquad g'(x) = 2x
	\]
	
	\hint
	Indsæt i kædereglen
	\[
	\frac{d}{dx} \left(x^2 + 1 \right)^5 = 5 \left(x^2 + 1 \right)^4 \cdot 2x = 10 x \cdot \left(x^2 + 1 \right)^4
	\]
	
\end{exercise}

\begin{exercise}{Differentiering 2 - 04}
	
	Bestem $\frac{d}{dx} \cos(2x)$.
	
	\answerbox{-2 \sin(2x)}
	
	\hint
	Benyt kæde reglen
	\[
	\frac{d}{dx} f(g(x)) = f'(g(x)) \cdot g'(x)
	\]
	
	\hint
	Sæt $f(x) = \cos(x)$ og $g(x) = 2x$ og bestem $f'(x)$ og $g'(x)$.
	\[
	f'(x) = - \sin(x) \qquad g'(x) = 2
	\]
	
	\hint
	Indsæt i kædereglen
	\[
	\frac{d}{dx} \cos(2x) = -\sin(2x) \cdot 2 = -2 \sin(2x)
	\]
	
\end{exercise}

\begin{exercise}{Differentiering 2 - 05}
	
	Bestem $\frac{d}{dx} e^{3x + x^5}$.
	
	\answerbox{e^{3x + x^5} \cdot (5x^4 + 3)}
	
	\hint
	Benyt kæde reglen
	\[
	\frac{d}{dx} f(g(x)) = f'(g(x)) \cdot g'(x)
	\]
	
	\hint
	Sæt $f(x) = e^x$ og $g(x) = 3x + x^5$ og bestem $f'(x)$ og $g'(x)$.
	\[
	f'(x) = e^x \qquad g'(x) = 3 + 5 x^4
	\]
	
	\hint
	Indsæt i kædereglen
	\[
	\frac{d}{dx} e^{3x + x^5} = e^{3x + x^5} \cdot (3 + 5x^4)
	\]
	
\end{exercise}

\begin{exercise}{Differentiering 2 - 06}
	
	Bestem $\frac{d}{dx} \sqrt{x+3}$.
	
	\answerbox{\frac{1}{2 \sqrt{x+3}}}
	
	\hint
	Benyt kæde reglen
	\[
	\frac{d}{dx} f(g(x)) = f'(g(x)) \cdot g'(x)
	\]
	
	\hint
	Sæt $f(x) = \sqrt{x}$ og $g(x) = x+3$ og bestem $f'(x)$ og $g'(x)$.
	\[
	f'(x) =\frac{1}{2 \sqrt{x}} \qquad g'(x) = 1 
	\]
	
	\hint
	Indsæt i kædereglen
	\[
	\frac{d}{dx} \sqrt{x+3} = \frac{1}{2 \sqrt{x + 3}} \cdot 1  = \frac{1}{2 \sqrt{x + 3 }}
	\]
	
\end{exercise}

\begin{exercise}{Differentiering 2 - 07}
	
	Bestem $\frac{d}{dx} \ln(x^2)$.
	
	\answerbox{\frac{2}{x}}
	
	\hint
	Benyt kæde reglen
	\[
	\frac{d}{dx} f(g(x)) = f'(g(x)) \cdot g'(x)
	\]
	
	\hint
	Sæt $f(x) = \ln(x)$ og $g(x) = x^2$ og bestem $f'(x)$ og $g'(x)$.
	\[
	f'(x) = \frac{1}{x} \qquad g'(x) = 2x
	\]
	
	\hint
	Indsæt i kædereglen
	\[
	\frac{d}{dx} \ln(x^2) = \frac{1}{x^2} \cdot 2x = \frac{2}{x} 	
	\]
	
\end{exercise}

\begin{exercise}{Differentiering 2 - 08}
	
	Bestem $\frac{d}{dx} \sin(3x^2+1)$.
	
	\answerbox{6x \cos(3x^2 + 1)}
	
	\hint
	Benyt kæde reglen
	\[
	\frac{d}{dx} f(g(x)) = f'(g(x)) \cdot g'(x)
	\]
	
	\hint
	Sæt $f(x) = \sin(x)$ og $g(x) = 3x^2 + 1$ og bestem $f'(x)$ og $g'(x)$.
	\[
	f'(x) = \cos(x) \qquad g'(x) = 6x
	\]
	
	\hint
	Indsæt i kædereglen
	\[
	\frac{d}{dx} \sin(3x^2 + 1)  = \cos(3x^2 + 1) \cdot 6x 
	\]
	
\end{exercise}

\begin{exercise}{Differentiering 2 - 09}
	
	Bestem $\frac{d}{dx} \sqrt{x^3 + x^2 + 1}$.
	
	\answerbox{\frac{3x^2 + 2x}{2 \sqrt{x^3 + x^2 + 1}}}
	
	\hint
	Benyt kæde reglen
	\[
	\frac{d}{dx} f(g(x)) = f'(g(x)) \cdot g'(x)
	\]
	
	\hint
	Sæt $f(x) = \sqrt{x}$ og $g(x) = x^3 + x^2 + 1 $ og bestem $f'(x)$ og $g'(x)$.
	\[
	f'(x) = \frac{1}{2\sqrt{x}} \qquad g'(x) = 3x^2 + 2x
	\]
	
	\hint
	Indsæt i kædereglen
	\[
	\frac{d}{dx} \sqrt{x^3 + x^2 + 1} = \frac{1}{2 \sqrt{x^3 + x^2 + 1}} \cdot (3x^2 + 2x) = \frac{3x^2 + 2x}{2 \sqrt{x^3 + x^2 + 1}}
	\]
	
\end{exercise}

\begin{exercise}{Differentiering 2 - 10}
	
	Bestem $\frac{d}{dx} \frac{1}{x^2+2x}$.
	
	\answerbox{-\frac{2x+2}{(x^2+2x)^2}}
	
	\hint
	Benyt kæde reglen
	\[
	\frac{d}{dx} f(g(x)) = f'(g(x)) \cdot g'(x)
	\]
	
	\hint
	Sæt $f(x) = \frac{1}{x}$ og $g(x) = x^2 + 2x$ og bestem $f'(x)$ og $g'(x)$.
	\[
	f'(x) = - \frac{1}{x^2} \qquad g'(x) = 2x + 2
	\]
	
	\hint
	Indsæt i kædereglen
	\[
	\frac{d}{dx} \frac{1}{x^2+2x} = - \frac{1}{(x^2+2x)^2} \cdot (2x + 2 ) = - \frac{2x + 2}{(x^2 + 2x)^2}
	\]
	
\end{exercise}


\end{document}
